src/impl/internal.lean
@@ -1,4 +1,4 @@
-import impl.external
+import impl.state
 
 namespace Concrete
 
