src/refinement/requests.lean
@@ -1,4 +1,4 @@
-import impl.lookup
+import refinement.lookup
 
 namespace Refinement
 
