src/refinement/trace.lean
@@ -1,4 +1,4 @@
-import impl.simulation
+import refinement.simulation
 
 namespace Refinement
 
