src/refinement/wf.lean
@@ -1,4 +1,4 @@
-import impl.sweep
+import refinement.sweep
 
 namespace Refinement
 
